Reversed CRC32 spec.

specs/Spec.CRC32.fst
@@ -1,6 +1,7 @@
 module Spec.CRC32
 
 module BV = FStar.BitVector
+module Math = FStar.Math.Lib
 module Seq = FStar.Seq
 module U8 = FStar.UInt8
 module U32 = FStar.UInt32
@@ -8,36 +9,6 @@ module UInt = FStar.UInt
 
 open FStar.Seq
 open FStar.Mul
-
-private val do_u8_rev: BV.bv_t 8 -> (i: nat{i < 8}) -> (res: BV.bv_t 8) -> BV.bv_t 8
-let rec do_u8_rev s i res =
-  if i >= 1 then
-    do_u8_rev s (i - 1) (Seq.upd res (7 - i) (Seq.index s i))
-  else
-    Seq.upd res (7 - i) (Seq.index s i)
-
-private val do_uint_rev:
-    #n: nat{n > 0}
-  -> s: BV.bv_t n
-  -> i: nat{i < n}
-  -> res: BV.bv_t n{forall j. j > i ==> Seq.index res (n - j - 1) == Seq.index s j}
-  -> r: BV.bv_t n {forall j. Seq.index s j == Seq.index r (n - j - 1)}
-
-let rec do_uint_rev #n s i res =
-  if i >= 1 then
-    do_uint_rev s (i - 1) (Seq.upd res (n - i - 1) (Seq.index s i))
-  else
-    Seq.upd res (n - i - 1) (Seq.index s i)
-    
-let u8_rev v =
-  let s = UInt.to_vec (U8.v v) in
-  let emp = UInt.to_vec 0 in
-  U8.uint_to_t (UInt.from_vec (do_uint_rev s 7 emp))
-
-let u32_rev v =
-  let s = UInt.to_vec (U32.v v) in
-  let emp = UInt.to_vec 0 in
-  U32.uint_to_t (UInt.from_vec (do_uint_rev s 31 emp))
 
 let rec seq_append_index_l (#t: Type) (a b: Seq.seq t): Lemma
   (ensures forall i. i < Seq.length a ==> Seq.index a i == Seq.index (a @| b) i)
@@ -84,33 +55,64 @@ let logxor_vec_assoc (#n: nat{n > 0}) (a b c: BV.bv_t n): Lemma
   assert(Seq.equal (BV.logxor_vec (BV.logxor_vec a b) c) (BV.logxor_vec a (BV.logxor_vec b c)))
 
 #set-options "--z3rlimit 120 --z3seed 1"
-let poly_xor_zero_suffix (#n: nat{n >= 32}) (a: BV.bv_t n) (m: nat) (l: nat): Lemma
-  (ensures forall i. Seq.index (poly_xor (zero_vec_r m a)) i ==
-    Seq.index (poly_xor (zero_vec_r l a)) i) = ()
+let poly_xor_zero_prefix (#n: nat{n >= 32}) (a: BV.bv_t n) (m: nat{m > 0}): Lemma
+  (ensures forall (i: nat{i > 0}).
+    i < Seq.length (zero_vec_l m a) ==>
+    Seq.index (poly_xor (zero_vec_l m a)) i ==
+    Seq.index (poly_xor (zero_vec_l (m - 1) a)) (i - 1)) = ()
 
-let rec poly_xor_zero_vec_r (#n: nat{n >= 32}) (a: BV.bv_t n) (m: nat): Lemma
-  (ensures zero_vec_r m (poly_xor a) == poly_xor (zero_vec_r m a)) =
+let zero_vec_l_aux (#n: nat{n > 0}) (a: BV.bv_t n) (m: nat{m > 0}): Lemma
+  (ensures forall (i: nat{i > 0}).
+    i < Seq.length (zero_vec_l m a) ==>
+   Seq.index (zero_vec_l m a) i == Seq.index (zero_vec_l (m - 1) a) (i - 1)) = ()
+
+unfold let unsnoc (#a: Type) (s: Seq.seq a{
+  Seq.length s > 0
+}): Tot (res: Seq.seq a{
+  forall i.
+    Seq.length res == Seq.length s - 1 /\
+    (Seq.index s i == Seq.index res i)
+}) =
+  Seq.slice s 0 (Seq.length s - 1)
+
+unfold let last (#a: Type) (s: Seq.seq a{Seq.length s > 0}) =
+  Seq.index s (Seq.length s - 1)
+
+let rec poly_xor_zero_vec_l (#n: nat{n >= 32}) (a: BV.bv_t n) (m: nat): Lemma
+  (ensures zero_vec_l m (poly_xor a) == poly_xor (zero_vec_l m a)) =
   match m with
   | 0 -> ()
   | _ ->
-    let b = zero_vec_r m (poly_xor a) in
-    let c = poly_xor (zero_vec_r m a) in
-    let b' = zero_vec_r (m - 1) (poly_xor a) in
-    let c' = poly_xor (zero_vec_r (m - 1) a) in
-    poly_xor_zero_suffix a m (m - 1);
-    poly_xor_zero_vec_r a (m - 1);
-    assert(forall i. Seq.index b i == Seq.index b' i);
-    assert(forall i. Seq.index c i == Seq.index c' i);
-    assert(Seq.index b (m + n - 1) == Seq.index c (m + n - 1));
+    let b = zero_vec_l m (poly_xor a) in
+    let c = poly_xor (zero_vec_l m a) in
+    let b' = zero_vec_l (m - 1) (poly_xor a) in
+    let c' = poly_xor (zero_vec_l (m - 1) a) in
+    let p = poly (n + m + 1) in
+    let p' = unsnoc p in
+    poly_xor_zero_prefix a m;
+    zero_vec_l_aux (poly_xor a) m;
+    poly_xor_zero_vec_l a (m - 1);
+    calc (==) {
+      Seq.index c 0;
+      =={}
+      Seq.index ((zero_vec_l m a) -@ p') 0;
+      =={
+        assert(Seq.index (zero_vec_l m a) 0 == false);
+        assert(Seq.index p 0 == false);
+        assert(Seq.index p' 0 == false)
+      }
+      false;
+    };
+    assert(Seq.index b 0 == Seq.index c 0);
     assert(Seq.equal b c)
 
 let poly_xor_sub_eq (#n: nat{n > 32}) (a: BV.bv_t n): Lemma
-  (ensures poly_xor #(n - 1) (Seq.tail a) == Seq.tail (a -@ (poly n))) =
-  assert(Seq.equal (poly_xor #(n - 1) (Seq.tail a)) (Seq.tail (a -@ (poly n))))
+  (ensures poly_xor #(n - 1) (unsnoc a) == unsnoc (a -@ (poly n))) =
+  assert(Seq.equal (poly_xor #(n - 1) (unsnoc a)) (unsnoc (a -@ (poly n))))
 
 let poly_xor_aux (#n: nat{n >= 32}) (a b: BV.bv_t n): Lemma
   (ensures (poly_xor a) +@ (poly_xor b) == a +@ b) =
-  let p' = Seq.tail (poly (n + 1)) in
+  let p' = unsnoc (poly (n + 1)) in
   calc (==) {
     (poly_xor a) +@ (poly_xor b);
     =={}
@@ -128,45 +130,45 @@ let rec poly_mod_zero (#n: nat{n > 32}) (a: BV.bv_t n {a == BV.zero_vec #n}): Le
   match n with
   | 33 -> assert_norm(Seq.equal (poly_mod a) (BV.zero_vec #32))
   | _ -> 
-    assert_norm(Seq.equal (Seq.tail a) (BV.zero_vec #(n - 1)));
-    poly_mod_zero #(n - 1) (Seq.tail a)
+    assert_norm(Seq.equal (unsnoc a) (BV.zero_vec #(n - 1)));
+    poly_mod_zero #(n - 1) (unsnoc a)
 
 let rec poly_mod_add (#n: nat{n > 32}) (a b: BV.bv_t n): Lemma
   (ensures (poly_mod a) +@ (poly_mod b) == poly_mod (a +@ b)) =
-  let a' = Seq.tail a in
-  let b' = Seq.tail b in
+  let a' = unsnoc a in
+  let b' = unsnoc b in
   let c = a +@ b in
   let c' = gf2_plus #(n - 1) a' b' in
 
-  if Seq.head a = Seq.head b then
-    assert(Seq.equal (Seq.tail c) c')
+  if last a = last b then
+    assert(Seq.equal (unsnoc c) c')
   else
-    assert(Seq.head a <> Seq.head b);
+    assert(last a <> last b);
 
   if n = 33 then begin
-    if Seq.head a then assert(Seq.equal (poly_mod a) (poly_xor #32 a')) else ();
-    if Seq.head b then assert(Seq.equal (poly_mod b) (poly_xor #32 b')) else ();
+    if last a then assert(Seq.equal (poly_mod a) (poly_xor #32 a')) else ();
+    if last b then assert(Seq.equal (poly_mod b) (poly_xor #32 b')) else ();
     
-    match Seq.head a = Seq.head b with
-    | true -> if Seq.head a then poly_xor_aux #32 a' b' else ()
+    match last a = last b with
+    | true -> if last a then poly_xor_aux #32 a' b' else ()
     | false -> assert(Seq.equal (poly_mod c) (poly_xor c'))
   end else begin
     assert(n > 33);
-    if Seq.head a then begin
-      assert(Seq.equal (Seq.tail (a -@ (poly n))) (poly_xor #(n - 1) a'));
+    if last a then begin
+      assert(Seq.equal (unsnoc (a -@ (poly n))) (poly_xor #(n - 1) a'));
       assert_norm(poly_mod a == poly_mod (poly_xor #(n - 1) a'))
     end else
       assert_norm(poly_mod a == poly_mod #(n - 1) a');
 
-    if Seq.head b then begin
-      assert(Seq.equal (Seq.tail (b -@ (poly n))) (poly_xor #(n - 1) b'));
+    if last b then begin
+      assert(Seq.equal (unsnoc (b -@ (poly n))) (poly_xor #(n - 1) b'));
       assert_norm(poly_mod b == poly_mod (poly_xor #(n - 1) b'))
     end else
       assert_norm(poly_mod b == poly_mod #(n - 1) b');
 
-    match Seq.head a = Seq.head b with
+    match last a = last b with
     | true ->
-      if Seq.head a then
+      if last a then
         let a'' = poly_xor #(n - 1) a' in
         let b'' = poly_xor #(n - 1) b' in
         calc (==) {
@@ -191,12 +193,18 @@ let rec poly_mod_add (#n: nat{n > 32}) (a b: BV.bv_t n): Lemma
           poly_mod c;
         }
     | false ->
-      assert(Seq.equal (poly_mod c) (poly_mod (poly_xor c')));
-      let x = if Seq.head a then a else b in
-      let x' = Seq.tail x in
-      let y = if Seq.head a then b else a in
-      let y' = Seq.tail y in
-      let p' = Seq.tail (poly n) in
+      calc (==) {
+        poly_mod c;
+        =={assert(last c == true)}
+        poly_mod #(n - 1) (unsnoc (c -@ poly n));
+        =={assert(Seq.equal (unsnoc (c -@ poly n)) (poly_xor #(n - 1) c'))}
+        poly_mod (poly_xor #(n - 1) c');
+      };
+      let x = if last a then a else b in
+      let x' = unsnoc x in
+      let y = if last a then b else a in
+      let y' = unsnoc y in
+      let p' = unsnoc (poly n) in
       calc (==) {
         (poly_mod x) +@ (poly_mod y);
         =={}
@@ -209,12 +217,14 @@ let rec poly_mod_add (#n: nat{n > 32}) (a b: BV.bv_t n): Lemma
   end
 
 unfold let magic_matrix_pattern (nzeros: nat{nzeros > 0}) (i: nat{i < 32}):
-  res: BV.bv_t (32 + nzeros){
-    forall j. (j == i ==> Seq.index res j == true) /\ (j <> i ==> Seq.index res j == false)
+  res: BV.bv_t (nzeros + 32){
+    forall j.
+      (j == nzeros + 31 - i ==> Seq.index res j == true) /\
+      (j <> nzeros + 31 - i ==> Seq.index res j == false)
   } =
-  let zero_right = BV.zero_vec #(nzeros + 32 - i - 1) in
-  let one = ones_vec_l 1 zero_right in
-  zero_vec_l i one
+  let zero_left = BV.zero_vec #(nzeros + 32 - i - 1) in
+  let one = ones_vec_r 1 zero_left in
+  zero_vec_r i one
 
 unfold let is_magic_matrix_elem (nzeros: nat{nzeros > 0}) (i: nat {i < 32}) (v: BV.bv_t 32) =
   poly_mod (magic_matrix_pattern nzeros i) == v
@@ -232,12 +242,12 @@ val magic_matrix_init: s: sub_matrix_t 1 -> Tot (matrix_t 1) (decreases 32 - (Se
 let rec magic_matrix_init s =
   let l = Seq.length s in
   if l = 0 then begin
-    let m = ones_vec_l 1 (BV.zero_vec #32) in
+    let m = ones_vec_r 1 (BV.zero_vec #32) in
     let n = poly_xor (BV.zero_vec #32) in
     calc (==) {
       poly_mod #33 m;
-      =={assert(Seq.head m == true)}
-      Seq.tail (m -@ poly 33);
+      =={assert(last m == true)}
+      unsnoc (m -@ poly 33);
       =={}
       n;
     };
@@ -264,35 +274,38 @@ let rec magic_matrix_init s =
   end else 
     s
 
-type matrix_dividend (nzeros: nat{nzeros > 0}) = d: BV.bv_t (32 + nzeros) {
-  forall i. i > 31 /\ i < Seq.length d ==> Seq.index d i == false
+type matrix_dividend (nzeros: nat{nzeros > 0}) = d: BV.bv_t (nzeros + 32) {
+  forall i. i < nzeros ==> Seq.index d i == false
 }
 
 val bit_extract:
     #nzeros: nat{nzeros > 0}
   -> n: matrix_dividend nzeros
   -> i: nat{i < 32}
-  -> res: BV.bv_t (32 + nzeros) {
-      forall j. (j == i ==> Seq.index res j == Seq.index n j) /\
-        (j <> i ==> Seq.index res j == false)
+  -> res: BV.bv_t (nzeros + 32) {
+      forall j.
+        (j == nzeros + 31 - i ==> Seq.index res j == Seq.index n j) /\
+        (j <> nzeros + 31 - i ==> Seq.index res j == false)
     }
 
 let bit_extract #nzeros n i =
-  let zero_right = BV.zero_vec #(nzeros + 32 - i - 1) in
-  let bit = (Seq.create 1 (Seq.index n i)) @| zero_right in
-  zero_vec_l #(nzeros + 32 - i) i bit
+  let zero_left = BV.zero_vec #(nzeros + 32 - i - 1) in
+  let bit = zero_left @| (Seq.create 1 (Seq.index n (nzeros + 31 - i))) in
+  zero_vec_r #(nzeros + 32 - i) i bit
 
 val bit_sum:
     #nzeros: nat{nzeros > 0}
   -> n: matrix_dividend nzeros
   -> i: nat{i < 32}
-  -> res: BV.bv_t (32 + nzeros) {
-    forall j. (j <= i ==> Seq.index res j == Seq.index n j) /\ (j > i ==> Seq.index res j == false)
+  -> res: BV.bv_t (nzeros + 32) {
+    forall j.
+      (j >= nzeros + 31 - i ==> Seq.index res j == Seq.index n j) /\
+      (j < nzeros + 31 - i ==> Seq.index res j == false)
   }
 
 let rec bit_sum #nzeros n i =
   match i with
-  | 0 -> bit_extract n i
+  | 0 -> bit_extract #nzeros n i
   | _ -> (bit_extract n i) +@ (bit_sum n (i - 1))
 
 val do_magic_matrix_times:
@@ -301,16 +314,17 @@ val do_magic_matrix_times:
   -> n: BV.bv_t 32
   -> i: nat{i < 32}
   -> res: BV.bv_t 32{
-      res == poly_mod (bit_extract (zero_vec_r nzeros n) i)
+      res == poly_mod (bit_extract #nzeros (zero_vec_l nzeros n) i)
     }
 
-let do_magic_matrix_times
-  (#nzeros: nat{nzeros > 0}) (m: matrix_t nzeros) (n: BV.bv_t 32) (i: nat{i < 32}) =
-  if Seq.index n i then begin
+let do_magic_matrix_times #nzeros m n i =
+  let pat = magic_matrix_pattern nzeros i in
+  let ext = bit_extract #nzeros (zero_vec_l nzeros n) i in
+  if Seq.index n (31 - i) then begin
     Seq.index m i
   end else begin
-    assert(Seq.equal (bit_extract (zero_vec_r nzeros n) i) (BV.zero_vec #(32 + nzeros)));
-    poly_mod_zero (bit_extract (zero_vec_r nzeros n) i);
+    assert(Seq.equal ext (BV.zero_vec #(nzeros + 32)));
+    poly_mod_zero ext;
     BV.zero_vec #32
   end
 
@@ -320,7 +334,7 @@ val magic_matrix_times':
   -> n: BV.bv_t 32
   -> i: nat{i < 32}
   -> res: BV.bv_t 32{
-    res == poly_mod (bit_sum (zero_vec_r nzeros n) i)
+    res == poly_mod (bit_sum #nzeros (zero_vec_l nzeros n) i)
   }
 
 let rec magic_matrix_times'
@@ -329,76 +343,80 @@ let rec magic_matrix_times'
   | 0 -> do_magic_matrix_times m n i
   | _ -> 
     let n' = do_magic_matrix_times m n i in
-    poly_mod_add (bit_extract (zero_vec_r nzeros n) i) (bit_sum (zero_vec_r nzeros n) (i - 1));
+    let e = bit_extract #nzeros (zero_vec_l nzeros n) i in
+    let sum = bit_sum #nzeros (zero_vec_l nzeros n) (i - 1) in
+    poly_mod_add e sum;
     n' +@ magic_matrix_times' m n (i - 1)
 
 val magic_matrix_times:
   #nzeros: nat {nzeros > 0} ->
   matrix_t nzeros ->
   n: BV.bv_t 32 ->
-  res: BV.bv_t 32 {res == poly_mod (zero_vec_r nzeros n)}
+  res: BV.bv_t 32 {res == poly_mod (zero_vec_l nzeros n)}
 
 let magic_matrix_times #nzeros m n =
-  assert_norm(Seq.equal (bit_sum (zero_vec_r nzeros n) 31) (zero_vec_r nzeros n));
+  assert(Seq.equal (bit_sum #nzeros (zero_vec_l nzeros n) 31) (zero_vec_l nzeros n));
   magic_matrix_times' m n 31
 
-#set-options "--z3rlimit 200"
-let rec poly_mod_zero_suffix (#n: nat{n > 32}) (a: BV.bv_t n) (m: nat{m > 0}): Lemma
-  (ensures poly_mod (zero_vec_r m (poly_mod a)) == poly_mod (zero_vec_r m a)) =
-  assert(Seq.equal (zero_vec_r #(n - 1) m (Seq.tail a)) (Seq.tail (zero_vec_r m a)));
+#set-options "--z3rlimit 200 --z3seed 1"
+let rec poly_mod_zero_prefix (#n: nat{n > 32}) (a: BV.bv_t n) (m: nat{m > 0}): Lemma
+  (ensures poly_mod (zero_vec_l m (poly_mod a)) == poly_mod (zero_vec_l m a)) =
+  assert(Seq.equal (zero_vec_l #(n - 1) m (unsnoc a)) (unsnoc (zero_vec_l m a)));
   if n = 33 then
-    if Seq.index a 0 then
+    if Seq.index a (n - 1) then
       calc (==) {
-        poly_mod (zero_vec_r m (poly_mod a));
-        =={assert(Seq.equal (poly_mod a) (poly_xor #(n - 1) (Seq.tail a)))}
-        poly_mod (zero_vec_r m (poly_xor #(n - 1) (Seq.tail a)));
+        poly_mod (zero_vec_l m (poly_mod a));
+        =={assert(Seq.equal (poly_mod a) (poly_xor #(n - 1) (unsnoc a)))}
+        poly_mod (zero_vec_l m (poly_xor #(n - 1) (unsnoc a)));
         =={
-          let left = (zero_vec_r m (poly_xor #(n - 1) (Seq.tail a))) in
-          let right = (poly_xor #(n + m - 1) (Seq.tail (zero_vec_r m a))) in
+          let left = (zero_vec_l m (poly_xor #(n - 1) (unsnoc a))) in
+          let right = (poly_xor #(n + m - 1) (unsnoc (zero_vec_l m a))) in
           assert(Seq.equal left right)
         }
-        poly_mod (poly_xor #(n + m - 1) (Seq.tail (zero_vec_r m a)));
-        =={poly_xor_sub_eq (zero_vec_r m a)}
-        poly_mod (zero_vec_r m a);
+        poly_mod (poly_xor #(n + m - 1) (unsnoc (zero_vec_l m a)));
+        =={poly_xor_sub_eq (zero_vec_l m a)}
+        poly_mod (zero_vec_l m a);
       }
     else
       calc (==) {
-        poly_mod (zero_vec_r m (poly_mod a));
+        poly_mod (zero_vec_l m (poly_mod a));
         =={}
-        poly_mod (zero_vec_r #(n - 1) m (Seq.tail a));
+        poly_mod (zero_vec_l #(n - 1) m (unsnoc a));
         =={}
-        poly_mod #(n + m - 1) (Seq.tail (zero_vec_r m a));
+        poly_mod #(n + m - 1) (unsnoc (zero_vec_l m a));
         =={}
-        poly_mod (zero_vec_r m a);
+        poly_mod (zero_vec_l m a);
       }
   else
-    if Seq.index a 0 then
+    if Seq.index a (n - 1) then
       calc (==) {
-        poly_mod (zero_vec_r m (poly_mod a));
+        poly_mod (zero_vec_l m (poly_mod a));
         =={}
-        poly_mod (zero_vec_r m (poly_mod #(n - 1) (Seq.tail (a -@ (poly n)))));
+        poly_mod (zero_vec_l m (poly_mod #(n - 1) (unsnoc (a -@ (poly n)))));
         =={poly_xor_sub_eq a}
-        poly_mod (zero_vec_r m (poly_mod (poly_xor #(n - 1) (Seq.tail a))));
-        =={poly_mod_zero_suffix (poly_xor #(n - 1) (Seq.tail a)) m}
-        poly_mod (zero_vec_r m (poly_xor #(n - 1) (Seq.tail a)));
-        =={poly_xor_zero_vec_r #(n - 1) (Seq.tail a) m}
-        poly_mod (poly_xor (zero_vec_r #(n - 1) m (Seq.tail a)));
+        poly_mod (zero_vec_l m (poly_mod (poly_xor #(n - 1) (unsnoc a))));
+        =={poly_mod_zero_prefix (poly_xor #(n - 1) (unsnoc a)) m}
+        poly_mod (zero_vec_l m (poly_xor #(n - 1) (unsnoc a)));
+        =={poly_xor_zero_vec_l #(n - 1) (unsnoc a) m}
+        poly_mod (poly_xor (zero_vec_l #(n - 1) m (unsnoc a)));
         =={}
-        poly_mod (poly_xor #(n + m - 1) (Seq.tail (zero_vec_r m a)));
-        =={poly_xor_sub_eq (zero_vec_r m a)}
-        poly_mod (zero_vec_r m a);
+        poly_mod (poly_xor #(n + m - 1) (unsnoc (zero_vec_l m a)));
+        =={poly_xor_sub_eq (zero_vec_l m a)}
+        poly_mod #(n + m - 1) (unsnoc ((zero_vec_l m a) -@ poly (n + m)));
+        =={assert(last (zero_vec_l m a) == true)}
+        poly_mod (zero_vec_l m a);
       }
     else
       calc (==) {
-        poly_mod (zero_vec_r m (poly_mod a));
+        poly_mod (zero_vec_l m (poly_mod a));
         =={}
-        poly_mod (zero_vec_r m (poly_mod #(n - 1) (Seq.tail a)));
-        =={poly_mod_zero_suffix #(n - 1) (Seq.tail a) m}
-        poly_mod (zero_vec_r #(n - 1) m (Seq.tail a));
+        poly_mod (zero_vec_l m (poly_mod #(n - 1) (unsnoc a)));
+        =={poly_mod_zero_prefix #(n - 1) (unsnoc a) m}
+        poly_mod (zero_vec_l #(n - 1) m (unsnoc a));
         =={}
-        poly_mod #(n + m - 1) (Seq.tail (zero_vec_r m a));
+        poly_mod #(n + m - 1) (unsnoc (zero_vec_l m a));
         =={}
-        poly_mod (zero_vec_r m a);
+        poly_mod (zero_vec_l m a);
       }
 
 let magic_matrix_times_double
@@ -406,22 +424,23 @@ let magic_matrix_times_double
   (ensures is_magic_matrix_elem (nzeros * 2) i (magic_matrix_times m (Seq.index m i))) =
   let p = magic_matrix_pattern nzeros i in
   let p' = magic_matrix_pattern (nzeros * 2) i in
-  let p'' = zero_vec_r nzeros p in
+  let p'' = zero_vec_l nzeros p in
   let n = magic_matrix_times m (Seq.index m i) in
-  poly_mod_zero_suffix p nzeros;
-  assert(forall j.{:pattern Seq.index p' j} j < 32 + nzeros ==> Seq.index p j == Seq.index p' j);
-  assert(forall j.{:pattern Seq.index p'' j} j < 32 + nzeros ==> Seq.index p j == Seq.index p'' j);
-  assert(forall j.{:pattern Seq.index p' j} j >= 32 + nzeros ==> Seq.index p' j == false);
-  assert(forall j.{:pattern Seq.index p'' j} j >= 32 + nzeros ==> Seq.index p'' j == false);
+  poly_mod_zero_prefix p nzeros;
+  assert(forall j.
+    j >= nzeros /\ j < nzeros * 2 + 32 ==>
+    Seq.index p (j - nzeros) == Seq.index p' j /\
+    Seq.index p (j - nzeros) == Seq.index p'' j);
+  assert(forall j. j < nzeros ==> Seq.index p' j == Seq.index p'' j);
   assert(Seq.equal p'' p');
   calc (==) {
     n;
     =={}
-    poly_mod (zero_vec_r nzeros (Seq.index m i));
+    poly_mod (zero_vec_l nzeros (Seq.index m i));
     =={}
-    poly_mod (zero_vec_r nzeros (poly_mod p));
+    poly_mod (zero_vec_l nzeros (poly_mod p));
     =={}
-    poly_mod (zero_vec_r nzeros p);
+    poly_mod (zero_vec_l nzeros p);
     =={}
     poly_mod p';
     =={}
@@ -438,7 +457,7 @@ val magic_matrix_square':
 let rec magic_matrix_square' #nzeros m s =
   if Seq.length s < 32 then begin
     magic_matrix_times_double m (Seq.length s);
-    let n: BV.bv_t 32 = magic_matrix_times m (Seq.index m (Seq.length s)) in
+    let n = magic_matrix_times m (Seq.index m (Seq.length s)) in
     let res = s @| (Seq.create 1 n) in
     seq_append_index_r s (Seq.create 1 n);
     calc (==) {
